added Free code

Test/civl/alloc.bpl
@@ -11,21 +11,26 @@ axiom (forall x: [int]bool, y: [int]int :: {cons(x,y)} dom(cons(x, y)) == x && m
 function EmptyLmap(): (lmap);
 axiom (dom(EmptyLmap()) == MapConstBool(false));
 
-function Add(x: lmap, i: int, v: int): (lmap);
-axiom (forall x: lmap, i: int, v: int :: dom(Add(x, i, v)) == dom(x)[i:=true] && map(Add(x, i, v)) == map(x)[i := v]);
+function Add(x: lmap, i: int): (lmap);
+axiom (forall x: lmap, i: int :: dom(Add(x, i)) == dom(x)[i:=true] && map(Add(x, i)) == map(x));
 
 function Remove(x: lmap, i: int): (lmap);
 axiom (forall x: lmap, i: int :: dom(Remove(x, i)) == dom(x)[i:=false] && map(Remove(x, i)) == map(x));
 
+function {:inline} PoolInv(unallocated:[int]bool, pool: lmap) : (bool)
+{
+    (forall x: int :: unallocated[x] ==> dom(pool)[x])
+}
+
 procedure {:yields} {:layer 2} Main()
-requires {:layer 1} (forall x: int :: unallocated[x] ==> dom(pool)[x]);
-ensures {:layer 1} (forall x: int :: unallocated[x] ==> dom(pool)[x]);
+requires {:layer 1} PoolInv(unallocated, pool);
+ensures {:layer 1} PoolInv(unallocated, pool);
 {
    var {:layer 1} {:linear "mem"} l: lmap;
    var i: int;
    par Yield() | Dummy();
    while (*)
-   invariant {:layer 1} (forall x: int :: unallocated[x] ==> dom(pool)[x]);
+   invariant {:layer 1} PoolInv(unallocated, pool);
    {
       call  l, i := Alloc();
       async call Thread(l, i);
@@ -35,8 +40,8 @@ ensures {:layer 1} (forall x: int :: unallocated[x] ==> dom(pool)[x]);
 }
 
 procedure {:yields} {:layer 2} Thread({:layer 1} {:linear_in "mem"} local_in: lmap, i: int)
-requires {:layer 1} (forall x: int :: unallocated[x] ==> dom(pool)[x]);
-ensures {:layer 1} (forall x: int :: unallocated[x] ==> dom(pool)[x]);
+requires {:layer 1} PoolInv(unallocated, pool);
+ensures {:layer 1} PoolInv(unallocated, pool);
 requires {:layer 1} dom(local_in)[i] && map(local_in)[i] == mem[i];
 requires {:layer 2} dom(local_in)[i];
 {
@@ -50,13 +55,13 @@ requires {:layer 2} dom(local_in)[i];
     call o := Read(local, i);
     assert {:layer 2} o == 42;
     while (*)
-    invariant {:layer 1} (forall x: int :: unallocated[x] ==> dom(pool)[x]);
+    invariant {:layer 1} PoolInv(unallocated, pool);
     {
         call l, y := Alloc();
         call l := Write(l, y, 42);
 	call o := Read(l, y);
 	assert {:layer 2} o == 42;
-        call Free(l);
+        call Free(l, y);
 	par Yield() | Dummy();
     }
     par Yield() | Dummy();
@@ -68,8 +73,8 @@ procedure {:pure} {:inline 1} Copy({:linear_in "mem"} l: lmap) returns ({:linear
 }
 
 procedure {:yields} {:layer 1,2} Alloc() returns ({:layer 1} {:linear "mem"} l: lmap, i: int)
-requires {:layer 1} (forall x: int :: unallocated[x] ==> dom(pool)[x]);
-ensures {:layer 1} (forall x: int :: unallocated[x] ==> dom(pool)[x]);
+requires {:layer 1} PoolInv(unallocated, pool);
+ensures {:layer 1} PoolInv(unallocated, pool);
 ensures {:layer 1} dom(l)[i] && map(l)[i] == mem[i];
 ensures {:right} |{ A: assume dom(l)[i]; return true; }|;
 {
@@ -79,17 +84,21 @@ ensures {:right} |{ A: assume dom(l)[i]; return true; }|;
     call YieldMem(l, i);
 }
 
-procedure {:yields} {:layer 1,2} Free({:layer 1} {:linear_in "mem"} l: lmap)
-requires {:layer 1} (forall x: int :: unallocated[x] ==> dom(pool)[x]);
-ensures {:layer 1} (forall x: int :: unallocated[x] ==> dom(pool)[x]);
+procedure {:yields} {:layer 1,2} Free({:layer 1} {:linear_in "mem"} l: lmap, i: int)
+requires {:layer 1} PoolInv(unallocated, pool);
+ensures {:layer 1} PoolInv(unallocated, pool);
+requires {:layer 1} dom(l)[i];
 ensures {:both} |{ A: return true; }|;
 {
+    call Yield();
+    call FreeLinear(l, i);
+    call ReturnAddr(i);
     call Yield();
 }
 
 procedure {:yields} {:layer 1,2} Read({:layer 1} {:linear "mem"} l: lmap, i: int) returns (o: int)
-requires {:layer 1} (forall x: int :: unallocated[x] ==> dom(pool)[x]);
-ensures {:layer 1} (forall x: int :: unallocated[x] ==> dom(pool)[x]);
+requires {:layer 1} PoolInv(unallocated, pool);
+ensures {:layer 1} PoolInv(unallocated, pool);
 requires {:layer 1} dom(l)[i] && map(l)[i] == mem[i];
 ensures {:both} |{ A: assert dom(l)[i]; o := map(l)[i]; return true; }|;
 {
@@ -99,8 +108,8 @@ ensures {:both} |{ A: assert dom(l)[i]; o := map(l)[i]; return true; }|;
 }
 
 procedure {:yields} {:layer 1,2} Write({:layer 1} {:linear_in "mem"} l: lmap, i: int, o: int) returns ({:layer 1} {:linear "mem"} l': lmap)
-requires {:layer 1} (forall x: int :: unallocated[x] ==> dom(pool)[x]);
-ensures {:layer 1} (forall x: int :: unallocated[x] ==> dom(pool)[x]);
+requires {:layer 1} PoolInv(unallocated, pool);
+ensures {:layer 1} PoolInv(unallocated, pool);
 requires {:layer 1} dom(l)[i] && map(l)[i] == mem[i];
 ensures {:layer 1} dom(l')[i] && map(l')[i] == mem[i];
 ensures {:both} |{ A: assert dom(l)[i]; l' := cons(dom(l), map(l)[i := o]); return true; }|;
@@ -116,26 +125,31 @@ modifies pool;
 requires dom(pool)[i];
 ensures pool == Remove(old(pool), i) && dom(l)[i] && map(l)[i] == mem[i];
 
+procedure {:layer 1} FreeLinear({:linear_in "mem"} l: lmap, i: int);
+modifies pool;
+requires !dom(pool)[i];
+ensures pool == Add(old(pool), i);
+
 procedure {:layer 1} WriteLinear({:layer 1} {:linear_in "mem"} l: lmap, i: int, o: int) returns ({:layer 1} {:linear "mem"} l': lmap);
 requires dom(l)[i];
 ensures l' == cons(dom(l), map(l)[i := o]);
 
 procedure {:yields} {:layer 1} Yield()
-requires {:layer 1} (forall x: int :: unallocated[x] ==> dom(pool)[x]);
-ensures {:layer 1} (forall x: int :: unallocated[x] ==> dom(pool)[x]);
+requires {:layer 1} PoolInv(unallocated, pool);
+ensures {:layer 1} PoolInv(unallocated, pool);
 {
     yield;
-    assert {:layer 1} (forall x: int :: unallocated[x] ==> dom(pool)[x]);
+    assert {:layer 1} PoolInv(unallocated, pool);
 }
 
 procedure {:yields} {:layer 1} YieldMem({:layer 1} {:linear "mem"} l: lmap, i: int)
-requires {:layer 1} (forall x: int :: unallocated[x] ==> dom(pool)[x]);
-ensures {:layer 1} (forall x: int :: unallocated[x] ==> dom(pool)[x]);
+requires {:layer 1} PoolInv(unallocated, pool);
+ensures {:layer 1} PoolInv(unallocated, pool);
 requires {:layer 1} dom(l)[i] && map(l)[i] == mem[i];
 ensures {:layer 1} dom(l)[i] && map(l)[i] == mem[i];
 {
     yield;
-    assert {:layer 1} (forall x: int :: unallocated[x] ==> dom(pool)[x]);
+    assert {:layer 1} PoolInv(unallocated, pool);
     assert {:layer 1} dom(l)[i] && map(l)[i] == mem[i];
 }
 
@@ -144,7 +158,7 @@ procedure {:yields} {:layer 2} Dummy()
     yield;
 }
 
-var {:layer 1, 1} pool: lmap;
+var {:layer 1, 1} {:linear "mem"} pool: lmap;
 var {:layer 0, 1} mem:[int]int;
 var {:layer 0, 1} unallocated:[int]bool;
 
@@ -156,3 +170,6 @@ ensures {:atomic} |{ A: mem[i] := o; return true; }|;
 
 procedure {:yields} {:layer 0, 1} PickAddr() returns (i: int);
 ensures {:atomic} |{ A: assume unallocated[i]; unallocated[i] := false; return true; }|;
+
+procedure {:yields} {:layer 0, 1} ReturnAddr(i: int);
+ensures {:atomic} |{ A: unallocated[i] := true; return true; }|;
